@prefix : <http://www.semanticweb.org/ioanna/ontologies/2018/4/untitled-ontology-275#> .
@prefix owl: <http://www.w3.org/2002/07/owl#> .
@prefix rdf: <http://www.w3.org/1999/02/22-rdf-syntax-ns#> .
@prefix xml: <http://www.w3.org/XML/1998/namespace> .
@prefix xsd: <http://www.w3.org/2001/XMLSchema#> .
@prefix rdfs: <http://www.w3.org/2000/01/rdf-schema#> .

<http://www.semanticweb.org/ioanna/ontologies/2018/4/untitled-ontology-275> a owl:Ontology ;
	<http://purl.org/dc/elements/1.1/creator> "Ioanna Kyvernitou, Mathieu d'Aquin, Marie-Louise Coolahan"^^xsd:string ;
	<http://purl.org/dc/elements/1.1/description> "The 'OntoSophia' ontology is written in OWL 2 DL. Its scope is to enable the formal characterisation of propositions, arguments, and quoted elements within the argumentative discussion in philosophical texts. Its structure follows the conceptual division between abstract arguments, abstract propositions and their expressions in texts, aiming to facilitate the representation of this division. This division enables to capture the cases where a restatement of an argument or proposition or a reference to the same argument or proposition occurs."^^xsd:string ;
	rdfs:comment ""@en ;
	<http://purl.org/dc/elements/1.1/title> "The 'OntoSophia' ontology"^^xsd:string ;
	<http://purl.org/dc/elements/1.1/date> "2018-05-18"^^xsd:string .
# 
# 
# #################################################################
# #
# #    Annotation properties
# #
# #################################################################
# 
# 
# http://purl.org/dc/elements/1.1/description

<http://purl.org/dc/elements/1.1/description> a owl:AnnotationProperty .
# 
# http://purl.org/dc/elements/1.1/subject

<http://purl.org/dc/elements/1.1/subject> a owl:AnnotationProperty ;
	rdfs:range <http://www.w3.org/2004/02/skos/core#Concept> .
# 
# http://purl.org/dc/terms/description

<http://purl.org/dc/terms/description> a owl:AnnotationProperty .
# 
# 
# 
# #################################################################
# #
# #    Object Properties
# #
# #################################################################
# 
# 
# http://purl.org/spar/cito/cites

<http://purl.org/spar/cito/cites> a owl:ObjectProperty ;
	rdfs:comment """Reused property from CiTO (http://purl.org/spar/cito/cites):The citing entity cites the cited entity, either directly and explicitly (as in the reference list of a journal article), indirectly (e.g. by citing a more recent paper by the same group on the same topic), or implicitly (e.g. as in artistic quotations or parodies, or in cases of plagiarism).
https://sparontologies.github.io/cito/current/cito.html#d4e118"""@en ;
	rdfs:label "cites"@en .
# 
# http://www.semanticweb.org/ioanna/ontologies/2018/4/untitled-ontology-275#contradicts

:contradicts a owl:ObjectProperty ;
	rdfs:domain :Argument , :ExpressionOfAProposition , :ExpressionOfAnArgument , :Proposition ;
	rdfs:range :Argument , :ExpressionOfAProposition , :ExpressionOfAnArgument , :Proposition ;
	rdfs:label "contradicts"@en .
# 
# http://www.semanticweb.org/ioanna/ontologies/2018/4/untitled-ontology-275#expresses

:expresses a owl:ObjectProperty , owl:FunctionalProperty ;
	rdfs:domain :ExpressionOfAProposition , :ExpressionOfAnArgument ;
	rdfs:range :Argument , :Proposition ;
	rdfs:label "expresses"@en .
# 
# http://www.semanticweb.org/ioanna/ontologies/2018/4/untitled-ontology-275#includes

:includes a owl:ObjectProperty ;
	rdfs:domain <http://purl.org/spar/deo/DiscourseElement> ;
	rdfs:range :ExpressionOfAProposition , :ExpressionOfAnArgument ;
	rdfs:label "includes"@en .
# 
# http://www.semanticweb.org/ioanna/ontologies/2018/4/untitled-ontology-275#reusedAs

:reusedAs a owl:ObjectProperty ;
	rdfs:comment "The property reusedAs designates that a Proposition, once justified in the text, is subsequently used as an Argument in support/contrast of another proposition within the discussion."@en ;
	rdfs:label "reusedAs"@en .
# 
# http://www.semanticweb.org/ioanna/ontologies/2018/4/untitled-ontology-275#supports

:supports a owl:ObjectProperty ;
	rdfs:domain :Argument , :ExpressionOfAProposition , :ExpressionOfAnArgument , :Proposition ;
	rdfs:range :Argument , :ExpressionOfAProposition , :ExpressionOfAnArgument , :Proposition ;
	rdfs:label "supports"@en .
# 
# http://www.w3.org/2004/02/skos/core#inScheme

<http://www.w3.org/2004/02/skos/core#inScheme> a owl:ObjectProperty ;
	rdfs:domain <http://www.w3.org/2004/02/skos/core#Concept> ;
	rdfs:range <http://www.w3.org/2004/02/skos/core#ConceptScheme> ;
	rdfs:comment "Reused property from the Simple Knowledge Organization System (SKOS):https://www.w3.org/2009/08/skos-reference/skos.html."@en .
# 
# 
# 
# #################################################################
# #
# #    Classes
# #
# #################################################################
# 
# 
# http://purl.org/spar/deo/DiscourseElement

<http://purl.org/spar/deo/DiscourseElement> a owl:Class ;
	rdfs:comment """Reused class from the Discourse Elements Ontology (DEO) to represent the document part of the resource which carries out a rhetorical function.

https://sparontologies.github.io/deo/current/deo.html#d4e325"""@en ;
	rdfs:label "Discourse Element"@en .
# 
# http://www.semanticweb.org/ioanna/ontologies/2018/4/untitled-ontology-275#Argument

:Argument a owl:Class ;
	owl:disjointWith :Proposition ;
	rdfs:comment "It represents the description of an abstract statement of the reasons for and against a proposition, which has different expressions in texts."^^rdfs:Literal ;
	rdfs:label "Argument"@en .
# 
# http://www.semanticweb.org/ioanna/ontologies/2018/4/untitled-ontology-275#Definition

:Definition a owl:Class ;
	rdfs:subClassOf :Proposition ;
	rdfs:comment "It represents what a philosophical concept means as defined by different authors and texts."@en ;
	rdfs:label "Definition"@en .
# 
# http://www.semanticweb.org/ioanna/ontologies/2018/4/untitled-ontology-275#ExpressionOfAProposition

:ExpressionOfAProposition a owl:Class ;
	rdfs:subClassOf _:genid1 .

_:genid1 a owl:Restriction ;
	owl:onProperty :expresses ;
	owl:allValuesFrom :Proposition .

:ExpressionOfAProposition owl:disjointWith :ExpressionOfAnArgument ;
	rdfs:comment "It refers to an expression, i.e formulation of an abstract proposition in a text."@en ;
	rdfs:label "Expression of a proposition"@en .
# 
# http://www.semanticweb.org/ioanna/ontologies/2018/4/untitled-ontology-275#ExpressionOfAnArgument

:ExpressionOfAnArgument a owl:Class ;
	rdfs:subClassOf _:genid2 .

_:genid2 a owl:Restriction ;
	owl:onProperty :expresses ;
	owl:allValuesFrom :Argument .

:ExpressionOfAnArgument rdfs:comment "It captures the expression, i.e. formulation of an abstract argument."@en ;
	rdfs:label "Expression of an argument"@en .
# 
# http://www.semanticweb.org/ioanna/ontologies/2018/4/untitled-ontology-275#Proposition

:Proposition a owl:Class ;
	rdfs:comment "It refers to a statement or opinion, judgment or belief held to be true which is made justified by arguments."@en ;
	rdfs:label "Proposition"@en .
# 
# http://www.w3.org/2004/02/skos/core#Concept

<http://www.w3.org/2004/02/skos/core#Concept> a owl:Class ;
	rdfs:comment "Concept reused from https://www.w3.org/2009/08/skos-reference/skos.html."@en .
# 
# http://www.w3.org/2004/02/skos/core#ConceptScheme

<http://www.w3.org/2004/02/skos/core#ConceptScheme> a owl:Class ;
	rdfs:comment "Reused class from the Simple Knowledge Organization System (SKOS):https://www.w3.org/2009/08/skos-reference/skos.html."@en .
# 
# http://xmlns.com/foaf/0.1/Agent

<http://xmlns.com/foaf/0.1/Agent> a owl:Class ;
	rdfs:comment "An agent (eg. person, group, software or physical artifact), reused from FOAF:http://xmlns.com/foaf/spec/#term_Agent."@en ;
	rdfs:label "Agent"@en .
# 
# 
# 
# #################################################################
# #
# #    General axioms
# #
# #################################################################
# 
# 

_:genid3 a owl:AllDifferent ;
	owl:distinctMembers rdf:nil .
# 
# Generated by the OWL API (version 4.2.5.20160517-0735) https://github.com/owlcs/owlapi
